
# Ejercicio 1:

**1.**

$$
  y[n] - \frac{1}{2} y[n-1] + \frac{1}{4} y[n-2] = x[n]
$$

<br>

$$
  Y(z) - \frac{1}{2} Y(z) z^{-1} + \frac{1}{4} Y(z) z^{-2} = X(z)
$$

<br>

$$
  Y(z) ( 1 - \frac{1}{2} z^{-1} + \frac{1}{4} z^{-2}) = X(z)
$$

<br>

$$
H(z) = \frac{1}{1 - \frac{1}{2} z^{-1} + \frac{1}{4} z^{-2}}
$$
---

**2.**

$$
  y[n] = y[n-1] + y[n-2] + x[n-1]
$$

<br>


$$
  Y(z) ( 1 - z^{-1} - z^{-2}) = X(z) z^{-1}
$$

<br>


$$
  \frac{Y(z)}{X(z)} = \frac{z^{-1}}{1 - z^{-1} - z^{-2}}
$$

<br>


$$
  H(z) = \frac{z^{-1}}{1 - z^{-1} - z^{-2}}
$$

---

**3.**

$$
  y[n] = 7 x[n] + 2 y[n-1] - 6 y[n-2]
$$

<br>


$$
  Y(z) ( 1 - 2 z^{-1} + 6 z^{-2}) = 7 X(z) z^{-1}
$$

<br>


$$
  \frac{Y(z)}{X(z)} = \frac{7 z^{-1}}{1 - 2 z^{-1} + 6 z^{-2}}
$$

<br>


$$
  H(z) = \frac{7 z^{-1}}{1 - 2 z^{-1} + 6 z^{-2}}
$$

---

**4.**

$$
  y[n] = \sum \limits_{k=0}^{7} {2^{-k} x[n-k]}
$$

<br>


$$
  Y(z) = \sum \limits_{k=0}^{7} {2^{-k} z^{-k} X(z)}
$$

<br>


$$
  \frac{Y(z)}{X(z)} = \sum \limits_{k=0}^{7} {2^{-k} z^{-k}}
$$

<br>


$$
  H(z) = \sum \limits_{k=0}^{7} {2^{-k} z^{-k}}
$$
